Cleaned up notations a bit for ECCA with unicode, added refl and eqv to exp

ECCA/continuations.v
@@ -5,15 +5,13 @@ Require Import core_lemmas.
   ==--Continuation Typing--==
   ===========================*)
 
-(* TODO: incomplete *)
-
 Inductive cont: Type :=
   | Hole
   | LetHole (B: @exp (S 0))
 .
 Hint Constructors cont.
 Bind Scope ECCA_scope with cont.
-Notation "'[]'" := (Hole) (at level 200): ECCA_scope.
+Notation "'[⋅]'" := (Hole) (at level 200): ECCA_scope.
 
 Definition cont_is_ANF (k: cont): Prop :=
 match k with
@@ -31,28 +29,32 @@ Definition fill_hole (e: exp) (K: cont): exp:=
 end.
 Check fill_hole.
 Notation "'(' K ')' '[' N ']'" := (fill_hole N K) (at level 300): ECCA_scope.
-Notation "'LET' '[]' 'in' B" := (LetHole B) (at level 50) : ECCA_scope.
+Notation "'LET' '[⋅]' 'in' B" := (LetHole B) (at level 50) : ECCA_scope.
 
 Definition exId: @exp 1 := (eId (@bound 1 l0)).
-Definition example_aLetHole := (LET [] in (eId (@bound 1 l0)))%ECCA.
+Definition example_aLetHole := (LET [⋅] in (eId (@bound 1 l0)))%ECCA.
 Definition ex_fillhole := (fill_hole (eTru) example_aLetHole).
 Eval cbn in ex_fillhole.
 
 Inductive cont_type : Type :=
   | Cont (M A B: @exp 0)
 .
+Notation "'〔' M ':' A '〕' '⇒' B":= (Cont M A B) (at level 250, M at level 99). (* 〔 : \lbbrk, 〕: \rbbrk, ⇒ : \rArr *) 
 Hint Constructors cont_type.
 (* TODO: Add notation for cont type  *)
 
+
+
+Reserved Notation "g '⊩' K : T" (at level 250, K at level 99). (*⊩ : \Vdash *) 
 Inductive Types_cont : env -> cont  -> cont_type -> Prop :=
-  | aK_Empty (M: exp) (g: env) (A: exp):
-    Types g M A ->
-    Types_cont g Hole (Cont M A A)
-  | aK_Bind (g: env) (y: name) (M: exp) (M' A B: @exp 0):
-    Types g M' A ->
-    Types (ctx_cons g y (Def M' A)) (open y M) (open y (wk B)) ->
-    Types_cont g (LetHole M) (Cont M' A B)
-.
+  |  aK_Empty : forall (M : exp) (g : env) (A : exp),
+    (g ⊢ M : A)%ECCA ->
+    (g ⊩ ([]) : (〔M : A〕⇒ A))
+  | aK_Bind : forall (g : env) (y : name) (M M' A B : exp),
+    (g ⊢ M' : A) ->
+    (g & y ~ Def M' A ⊢ open y M : open y (wk B)) ->
+    (g ⊩ LET [⋅] in M : (〔M' : A〕⇒ B))
+where "g '⊩' K ':' T" := (Types_cont g K T) : ECCA_scope.
 
 Hint Constructors Types_cont.
 
@@ -92,20 +94,9 @@ Open Scope string.
 
 Function het_compose (K : cont) (M : exp) {measure esize M}: exp :=
   match M with
-  | eId _ => fill_hole M K
-  | eUni _ => fill_hole M K
-  | ePi _ _ => fill_hole M K
-  | eAbs _ _ => fill_hole M K
-  | eSig _ _ => fill_hole M K
-  | ePair _ _ _ => fill_hole M K
-  | eTru => fill_hole M K
-  | eFls => fill_hole M K
-  | eBool => fill_hole M K
   | eLet N M' => eLet N (close "k" (het_compose (shift_cont "k" K) (open "k" M')))
   | eIf v M1 M2 => eIf v (het_compose K M1) (het_compose K M2)
-  | eApp _ _ => fill_hole M K
-  | eFst _ => fill_hole M K
-  | eSnd _ => fill_hole M K
+  | _ => fill_hole M K
   end.
 Proof.
 + intros. cbn.
@@ -115,6 +106,7 @@ rewrite esize_open_id. cbn. lia.
 Qed.
 Hint Rewrite het_compose_equation.
 Check het_compose.
+
 
 Notation "K '《' M '》'" := (het_compose K M) (at level 50): ECCA_scope.
 
