ECCA/equiv.v
@@ -1,81 +1,82 @@
 Require Export reduction.
 
-Reserved Notation "g '|-' A '=e=' B"  (at level 250, A at level 99).
-Inductive Equiv: env -> exp -> exp -> Prop :=
-  | aE_Step (g: env) (e e1 e2: exp) :
-    RedClos g e1 e ->
-    RedClos g e2 e ->
-    Equiv g e1 e2
-  | aE_Reflect (g : env) (e1 e2 : exp) (x: var):
-    (has g x (Eq e1 e2)) -> (* stuff in the context needs a name even though eq shoudln't *)
-    Equiv g e1 e2
-  | aE_Subst (g: env) (M M1 M2: exp):
-    Equiv g M1 M2 ->
-    Equiv g (bind M1 M) (bind M2 M)
-  | aE_Refl (g: env) (M: exp):
-    Equiv g M M
-  | aE_Symm (g: env) (M M': exp):
-    Equiv g M' M ->
-    Equiv g M M'
-  | aE_Trans (g: env) (M1 M2 M': exp):
-    Equiv g M1 M' ->
-    Equiv g M' M2 ->
-    Equiv g M1 M2
-  | aE_Lam (g: env) (A A' M M': exp) (x: name):
-    Equiv g A A' ->
-    Equiv (g & x ~ (Assum A)) (open x M) (open x M') ->
-    Equiv g (eAbs A M) (eAbs A' M')
-  | aE_Eta1 (g: env) (A M M1 M2 M': exp) (x: name):
-    Equiv g M1 (eAbs A M) ->
-    Equiv g M2 M' ->
-    Equiv (g & x ~ (Assum A)) (open x M) (eApp M' (eId (free x))) ->
-    Equiv g M1 M2
-  | aE_Eta2 (g: env) (A M M1 M2 M': exp) (x: name):
-    Equiv g M1 M' ->
-    Equiv g M2 (eAbs A M) ->
-    Equiv (g & x ~ (Assum A)) (open x M) (eApp M' (eId (free x))) ->
-    Equiv g M1 M2
-  | aE_App (g: env) (V1 V1' V2 V2': exp): 
-    Equiv g V1 V1' ->
-    Equiv g V2 V2' ->
-    Equiv g (eApp V1 V2) (eApp V1' V2')
-  | aE_Pi (g: env) (A A' B B': exp) (x: name):
-    Equiv g A A' ->
-    Equiv (g & x ~ (Assum A)) (open x B) (open x B') ->
-    Equiv g (ePi A B) (ePi A' B')
-  | aE_Pair (g: env) (V1 V1' V2 V2' A A': exp):
-    Equiv g V1 V1' ->
-    Equiv g V2 V2' ->
-    Equiv g A A' ->
-    Equiv g (ePair V1 V2 A) (ePair V1' V2' A')
-  | aE_Fst (g: env) (V V': exp):
-    Equiv g V V' ->
-    Equiv g (eFst V) (eFst V')
-  | aE_Snd (g: env) (V V': exp):
-    Equiv g V V' ->
-    Equiv g (eSnd V) (eSnd V')
-  | aE_Sig (g: env) (A A' B B': exp) (x: name):
-    Equiv g A A' ->
-    Equiv (g & x ~ (Assum A)) (open x B) (open x B') ->
-    Equiv g (eSig A B) (eSig A' B')
-  | aE_Let (g: env) (N N' M M' A: exp) (x: name):
-    Equiv g N N' -> (* uh oh *)
-    Equiv (g & x ~ (Def N A)) (open x M) (open x M') ->
-    Equiv g (eLet N M) (eLet N' M')
-  | aE_If (g: env) (V V' M1 M1' M2 M2': exp) (x: name):
-    Equiv g V V' ->
-    Equiv (g & x ~ (Eq V eTru)) M1 M1' ->
-    Equiv (g & x ~ (Eq V eFls)) M2 M2' ->
-    Equiv g (eIf V M1 M2) (eIf V' M1' M2')
-  | aE_If_EtaTru (g: env) (V M1 M2: exp) (x: var):
-    (has g x (Eq V eTru)) ->
-    Equiv g (eIf V M1 M2) M1
-  | aE_If_EtaFls (g: env) (V M1 M2: exp) (x: var):
-    (has g x (Eq V eFls)) ->
-    Equiv g (eIf V M1 M2) M2
-  | aE_If2 (g: env) (V M: exp):
-    Equiv g (eIf V M M) M
-where "g '|-' A '=e=' B"  := (Equiv g A B): ECCA_scope.
+
+Reserved Notation "g '⊢' A '≡' B"  (at level 250, A at level 99). (*⊢ : \vdash , ≡ : \equiv *) 
+Inductive Equiv : env -> exp -> exp -> Prop :=
+  | aE_Step (g : env) (e e1 e2 : exp):
+      (g ⊢ e1 ⊳* e) -> 
+      (g ⊢ e2 ⊳* e) -> 
+      (g ⊢ e1 ≡ e2)
+  | aE_Reflect : forall (g : env) (e1 e2 : exp) (x : var),
+      assumes g x (eEqv e1 e2) -> 
+      (g ⊢ e1 ≡ e2)
+  | aE_Subst : forall (g : env) (M M1 M2 : exp),
+      (g ⊢ M1 ≡ M2) -> 
+      (g ⊢ bind M1 M ≡ bind M2 M)
+  | aE_Reflex : forall (g : env) (M : exp), 
+      (g ⊢ M ≡ M)
+  | aE_Symm : forall (g : env) (M M' : exp), 
+      (g ⊢ M' ≡ M) ->
+      (g ⊢ M ≡ M')
+  | aE_Trans : forall (g : env) (M1 M2 M' : exp),
+      (g ⊢ M1 ≡ M') -> 
+      (g ⊢ M' ≡ M2) -> 
+      (g ⊢ M1 ≡ M2)
+  | aE_Lam : forall (g : env) (A A' M M' : exp) (x : name),
+      (g ⊢ A ≡ A') ->
+      (g & x ~ Assum A ⊢ open x M ≡ open x M') ->
+      (g ⊢ eAbs A M ≡ eAbs A' M')
+  | aE_Eta1 : forall (g : env) (A M M1 M2 M' : exp) (x : name),
+      (g ⊢ M1 ≡ eAbs A M) ->
+      (g ⊢ M2 ≡ M') ->
+      (g & x ~ Assum A ⊢ open x M ≡ eApp M' (eId (free x))) -> 
+      (g ⊢ M1 ≡ M2)
+  | aE_Eta2 : forall (g : env) (A M M1 M2 M' : exp) (x : name),
+      (g ⊢ M1 ≡ M') ->
+      (g ⊢ M2 ≡ eAbs A M) ->
+      (g & x ~ Assum A ⊢ open x M ≡ eApp M' (eId (free x))) -> 
+      (g ⊢ M1 ≡ M2)
+  | aE_App : forall (g : env) (V1 V1' V2 V2' : exp),
+      (g ⊢ V1 ≡ V1') -> 
+      (g ⊢ V2 ≡ V2') -> 
+      (g ⊢ eApp V1 V2 ≡ eApp V1' V2')
+  | aE_Pi : forall (g : env) (A A' B B' : exp) (x : name),
+      (g ⊢ A ≡ A') ->
+      (g & x ~ Assum A ⊢ open x B ≡ open x B') -> 
+      (g ⊢ ePi A B ≡ ePi A' B')
+  | aE_Pair : forall (g : env) (V1 V1' V2 V2' A A' : exp),
+      (g ⊢ V1 ≡ V1') ->
+      (g ⊢ V2 ≡ V2') -> 
+      (g ⊢ A ≡ A') -> 
+      (g ⊢ ePair V1 V2 A ≡ ePair V1' V2' A')
+  | aE_Fst : forall (g : env) (V V' : exp), 
+      (g ⊢ V ≡ V') -> 
+      (g ⊢ eFst V ≡ eFst V')
+  | aE_Snd : forall (g : env) (V V' : exp), 
+      (g ⊢ V ≡ V') -> 
+      (g ⊢ eSnd V ≡ eSnd V')
+  | aE_Sig : forall (g : env) (A A' B B' : exp) (x : name),
+      (g ⊢ A ≡ A') ->
+      (g & x ~ Assum A ⊢ open x B ≡ open x B') -> 
+      (g ⊢ eSig A B ≡ eSig A' B')
+  | aE_Let : forall (g : env) (N N' M M' A : exp) (x : name),
+      (g ⊢ N ≡ N') ->
+      (g & x ~ Def N A ⊢ open x M ≡ open x M') -> 
+      (g ⊢ eLet N M ≡ eLet N' M')
+  | aE_If : forall (g : env) (V V' M1 M1' M2 M2' : exp) (p : name),
+      (g ⊢ V ≡ V') ->
+      (g & p ~ Assum (eEqv V eTru) ⊢ M1 ≡ M1') ->
+      (g & p ~ Assum (eEqv V eFls) ⊢ M2 ≡ M2') -> 
+      (g ⊢ eIf V M1 M2 ≡ eIf V' M1' M2')
+  | aE_If_EtaTru : forall (g : env) (V M1 M2 : exp) (p : var),
+      assumes g p (eEqv V eTru) -> 
+      (g ⊢ eIf V M1 M2 ≡ M1)
+  | aE_If_EtaFls : forall (g : env) (V M1 M2 : exp) (p : var),
+      assumes g p (eEqv V eFls) -> 
+      (g ⊢ eIf V M1 M2 ≡ M2)
+  | aE_If2 : forall (g : env) (V M : exp), 
+      (g ⊢ eIf V M M ≡ M)
+where "g '⊢' A '≡' B"  := (Equiv g A B): ECCA_scope.
 (*TODO: rewrite with notation for legibility*)
 Bind Scope ECCA_scope with Equiv.
 Hint Constructors Equiv.
