ECCA/typing.v
@@ -7,109 +7,117 @@ Require Export core_lemmas.
 *)
 
 (* TODO: Add notation for subtypes. *)
+Reserved Notation "g '⊢' A '≲' B"  (at level 250, A at level 99). (*⊢ : \vdash , ≲ : \less *) 
 Inductive SubTypes: env -> exp -> exp -> Prop :=
-| aST_Cong (g: env) (A B: exp) :
-  Equiv g A B ->
-  SubTypes g A B
-| aST_Cum (g: env) (i: nat) :
-  SubTypes g (eUni (uType i)) (eUni (uType (S i)))
-| aST_Pi (g: env) (A1 A2 B1 B2: exp) (x: name) :
-  (Equiv g A1 A2) ->
-  (SubTypes (g & x ~ Assum A2) (open x B1) (open x B2)) -> (* eId x1 ?*)
-  (SubTypes g (ePi A1 B1) (ePi A2 B2))
-| aST_Trans (g: env) (A A' B: exp) :
-  (SubTypes g A A') ->
-  (SubTypes g A' B) ->
-  (SubTypes g A B)
-| aST_Prop (g: env) :
-  (SubTypes g (eUni (uProp)) (eUni (uType 0)))
-| aST_Sig (g: env) (A1 A2 B1 B2: exp) (x: name):
-  (SubTypes g A1 A2) ->
-  (SubTypes (g & x ~ Assum A2) (open x B1) (open x B2)) ->
-  (SubTypes g (eSig A1 B1) (eSig A2 B2))
-.
+  | ST_Cong : forall (g : env) (A B : exp), 
+    (g ⊢ A ≡ B) -> 
+    (g ⊢ A ≲ B)
+  | ST_Cum : forall (g : env) (i : nat), 
+    (g ⊢ eUni (uType i) ≲ eUni (uType (S i)))
+  | ST_Pi : forall (g : env) (A1 A2 B1 B2 : exp) (x : name),
+    (g ⊢ A1 ≡ A2) ->
+    (g & x ~ Assum A2 ⊢ open x B1 ≲ open x B2) ->
+    (g ⊢ ePi A1 B1 ≲ ePi A2 B2)
+  | ST_Trans : forall (g : env) (A A' B : exp),
+    (g ⊢ A ≲ A') -> 
+    (g ⊢ A' ≲ B) -> (g ⊢ A ≲ B)
+  | ST_Prop : forall g : env, 
+    (g ⊢ eUni uProp ≲ eUni (uType 0))
+  | ST_Sig : forall (g : env) (A1 A2 B1 B2 : exp) (x : name),
+    (g ⊢ A1 ≲ A2) ->
+    (g & x ~ Assum A2 ⊢ open x B1 ≲ open x B2) ->
+    (g ⊢ eSig A1 B1 ≲ eSig A2 B2)
+where "g '⊢' a '≲' b" := (SubTypes g a b) : ECCA_scope.
+
+Print SubTypes.
 Hint Constructors SubTypes.
 
-Reserved Notation "g '|-' a ':' b" (at level 250, a at level 99).
+Reserved Notation "g '⊢' a ':' b" (at level 250, a at level 99).
+Reserved Notation "'⊢' g" (at level 250).
 Inductive Types: env -> exp -> exp -> Prop :=
 | aT_Ax_Prop (g: env) :
- (*  WellFormed g -> *)
-  (g |- (eUni uProp) : (eUni (uType 0)))
+  WellFormed g ->
+  (g ⊢ (eUni uProp) : (eUni (uType 0)))
 | aT_Ax_Type (g: env) (i: nat) :
-(*   WellFormed g -> *)
-  (g |- (eUni (uType i)) : (eUni (uType (S i))))
+  WellFormed g ->
+  (g ⊢ (eUni (uType i)) : (eUni (uType (S i))))
 | aT_Var (g: env) (x: atom) (A: exp) :
   (assumes g x A) -> (* this needs adjustment *)
-  (g |- (eId x) : A)
+  (g ⊢ (eId x) : A)
 | aT_Bool (g: env):
-(*   WellFormed g -> *)
-  (g |- (eBool) : (eUni (uType 0)))
+  WellFormed g ->
+  (g ⊢ (eBool) : (eUni (uType 0)))
 | aT_True (g: env):
-(*   WellFormed g -> *)
-  (g |- (eTru) : (eBool))
+  WellFormed g ->
+  (g ⊢ (eTru) : (eBool))
 | aT_False (g: env):
-(*   WellFormed g -> *)
-  (g |- (eFls) : (eBool)) 
+  WellFormed g ->
+  (g ⊢ (eFls) : (eBool)) 
 | aT_Sig (g: env) (x: name) (A B: exp) (i: nat) :
-  (g |- A : (eUni (uType i))) ->
-  ((g & x ~ Assum A) |- (open x B): (eUni (uType i))) ->
-  (g |- (eSig A B) : (eUni (uType i)))
+  (g ⊢ A : (eUni (uType i))) ->
+  ((g & x ~ Assum A) ⊢ (open x B): (eUni (uType i))) ->
+  (g ⊢ (eSig A B) : (eUni (uType i)))
 | aT_Pair (g: env) (v1 v2: exp) (A B: exp) :
-  (g |- v1 : A) ->
-  (g |- v2 : (bind v1 B)) ->
-  (g |- (ePair v1 v2 (eSig A B)) : (eSig A B))
+  (g ⊢ v1 : A) ->
+  (g ⊢ v2 : (bind v1 B)) ->
+  (g ⊢ (ePair v1 v2 (eSig A B)) : (eSig A B))
 | aT_Prod_Prop (g: env) (x: name) (A B: exp) (i: nat):
-  (g |- A : (eUni (uType i))) ->
+  (g ⊢ A : (eUni (uType i))) ->
   (Types (g & x ~ Assum A) (open x B) (eUni (uProp))) ->
-  (g |- (ePi A B) : (eUni (uProp)))
+  (g ⊢ (ePi A B) : (eUni (uProp)))
 | aT_Prod_Type (g: env) (x: name) (A B: exp) (i: nat):
-  (g |- A : (eUni (uType i))) ->
+  (g ⊢ A : (eUni (uType i))) ->
   (Types (g & x ~ Assum A) (open x B) (eUni (uType i))) ->
-  (g |- (ePi A B) : (eUni (uType i)))
+  (g ⊢ (ePi A B) : (eUni (uType i)))
 | aT_Lam (g: env) (x: name) (A e B: exp) :
   (Types (g & x ~ Assum A) (open x e) (open x B)) ->
-  (g |- (eAbs A e) : (ePi A B))
+  (g ⊢ (eAbs A e) : (ePi A B))
 | aT_Let (g: env) (n m A B: exp) (x: name):
-  (g |- n : A) ->
+  (g ⊢ n : A) ->
   (Types (g & x ~ Def n A) (open x m) (open x B)) ->
-  (g |- (eLet n m) : (bind n B))
-| aT_If (g: env) (B U e1 e2: exp) (e: exp) (x y: name):
-  ((g & x ~ Assum eBool) |- (open x B): U) -> 
-  (g |- e : eBool) ->
-  ((g & y ~ Eq e eTru) |- e1 : (bind eTru B)) ->
-  ((g & y ~ Eq e eFls) |- e2 : (bind eFls B)) -> 
-  (g |- (eIf e e1 e2) : (bind e B)) 
+  (g ⊢ (eLet n m) : (bind n B))
+| aT_If (g: env) (B U e1 e2: exp) (e: exp) (x p: name):
+  ((g & x ~ Assum eBool) ⊢ (open x B): U) -> 
+  (g ⊢ e : eBool) ->
+  ((g & p ~ (Assum (eEqv e eTru))) ⊢ e1 : (bind eTru B)) ->
+  ((g & p ~ (Assum (eEqv e eFls))) ⊢ e2 : (bind eFls B)) -> 
+  (g ⊢ (eIf e e1 e2) : (bind e B)) 
 | aT_Conv (g: env) (e A B U: exp) :
-  (g |- e : A) ->
-  (g |- B : U) ->
+  (g ⊢ e : A) ->
+  (g ⊢ B : U) ->
   (SubTypes g A B) ->
-  (g |- e : B)
+  (g ⊢ e : B)
 | aT_App (g: env) (x: name) (e e': exp) (A' B: exp) :
-  (g |- e : (ePi A' B)) ->
-  (g |- e' : A') ->
-  (g |- (eApp e e') : (bind e B))
+  (g ⊢ e : (ePi A' B)) ->
+  (g ⊢ e' : A') ->
+  (g ⊢ (eApp e e') : (bind e B))
 | aT_Fst (g: env) (e: exp) (A B: exp) :
-  (g |- e: (eSig A B)) ->
-  (g |- (eFst e): A)
+  (g ⊢ e: (eSig A B)) ->
+  (g ⊢ (eFst e): A)
 | aT_Snd (g: env) (e: exp) (A B: exp) :
-  (g |- e: (eSig A B)) ->
-  (g |- (eSnd e): (bind (eFst e) B)) 
-where "g '|-' a ':' b" := (Types g a b) : ECCA_scope
-(* with 
-(* ECCA Well-Formed Environments *)
+  (g ⊢ e: (eSig A B)) ->
+  (g ⊢ (eSnd e): (bind (eFst e) B)) 
+| aT_Refl (g: env) (e: exp) (A: exp):
+  (g ⊢ e: A) ->
+  (g ⊢ (eRefl e): (eEqv e e)) 
+| aT_Equiv (g: env) (A A': exp) (i: nat):
+  (g ⊢ A: (eUni (uType i))) ->
+  (g ⊢ A': (eUni (uType i))) ->
+  (g ⊢ (eEqv A A'): (eUni (uType i)))
+where "g '⊢' a ':' b" := (Types g a b) : ECCA_scope
+with (* ECCA Well-Formed Environments *)
 WellFormed: env -> Prop :=
-| wf_Empty:
-  WellFormed ctx_empty
-| wf_Assum (g: env) (x: name) (A U: exp) :
-  WellFormed g ->
-  Types g A U ->
-  WellFormed (g & x ~ Assum A)
-| wf_Def (g: env) (x: name) (e A U: exp) :
-  WellFormed g ->
-  Types g A U ->
-  Types g e A ->
-  WellFormed (g & x ~ Def e A) *)
-(* | W_Eq  *)
-.
-
+  |  wf_Empty : 
+    (⊢ ctx_empty)%ECCA
+  | wf_Assum : forall (g : env) (x : name) (A U : exp),
+    (⊢ g)%ECCA -> 
+    (g ⊢ A : U)%ECCA -> 
+    (⊢ g & x ~ Assum A)%ECCA
+  | wf_Def : forall (g : env) (x : name) (e A U : exp),
+    (⊢ g)%ECCA -> 
+    (g ⊢ A : U)%ECCA -> 
+    (g ⊢ e : A)%ECCA -> 
+    (⊢ g & x ~ Def e A)%ECCA
+where "'⊢' g" := (WellFormed g) : ECCA_scope.
 Hint Constructors Types.
+Hint Constructors WellFormed.
