ECCA/reduction.v
@@ -8,76 +8,77 @@ Require Export core.
 *)
 
 (* -Step- *)
-Inductive RedStep : env -> exp -> exp -> Prop :=
-  | R_ID (g: env) (x: atom) (e' A: exp) :
-    (has g x (Def e' A)) -> RedStep g (eId x) e'
-  | R_App (g: env) (A body arg: exp) :
-    RedStep g (eApp (eAbs A body) arg) (bind arg body) 
-  | R_Fst (g: env) (e1 e2 A: exp) :
-    RedStep g (eFst (ePair e1 e2 A)) e1
-  | R_Snd (g: env) (e1 e2 A: exp) :
-    RedStep g (eSnd (ePair e1 e2 A)) e2
-  | R_Let (g: env) (e1 e2: exp) :
-    RedStep g (eLet e1 e2) (bind e1 e2)  
-  | R_IfTru (g: env) (e1 e2: exp) :
-    RedStep g (eIf eTru e1 e2) e1
-  | R_IfFls (g: env) (e1 e2: exp) :
-    RedStep g (eIf eFls e1 e2) e2
-.
-Hint Constructors RedStep.
-Bind Scope ECCA_scope with RedStep.
+Reserved Notation "g '⊢' e1 '⊳' e2" (at level 250, e1 at level 99). (* ⊢ : \vdash , ⊳ : \RightTriangle *)
+Inductive Steps : env -> exp -> exp -> Prop :=
+  | st_ID (g: env) (x: atom) (e' A: exp) :
+    g ∋ x ~ Def e' A -> (g ⊢ eId x ⊳ e')
+  | st_App (g: env) (A body arg: exp) :
+    (g ⊢ eApp (eAbs A body) arg ⊳ bind arg body)
+  | st_Fst (g: env) (e1 e2 A: exp) :
+    (g ⊢ eFst (ePair e1 e2 A) ⊳ e1)
+  | st_Snd (g: env) (e1 e2 A: exp) :
+    (g ⊢ eSnd (ePair e1 e2 A) ⊳ e2)
+  | st_Let (g: env) (e1 e2: exp) :
+    (g ⊢ eLet e1 e2 ⊳ bind e1 e2)  
+  | st_IfTru (g: env) (e1 e2: exp) :
+    (g ⊢ eIf eTru e1 e2 ⊳ e1)
+  | st_IfFls (g: env) (e1 e2: exp) :
+    (g ⊢ eIf eFls e1 e2 ⊳ e2)
+where "g '⊢' e1 '⊳' e2":= (Steps g e1 e2): ECCA_scope.
+Check st_Let. Check st_IfTru. Check st_IfFls.
+Hint Constructors Steps.
+Bind Scope ECCA_scope with Steps.
 
-
-
-(* Reflective Transitive Closure of step*)
-Inductive RedClos : env -> exp -> exp -> Prop :=
+(* Congruence Conversion Rules*)
+Reserved Notation "g '⊢' e1 '⊳*' e2" (at level 250, e1 at level 99). (* ⊢ : \vdash , ⊳ : \RightTriangle *) 
+Inductive Reduces : env -> exp -> exp -> Prop :=
   | R_RedR (g: env) (e e': exp): (* maybe don't need this one? it follows from refl + trans*)
-      RedStep g e e' ->
-      RedClos g e e'
-  | R_Refl (g: env) (e: exp):
-      RedClos g e e
+      (Steps g e e') ->
+      (g ⊢ e ⊳* e')
+  | R_Reflex (g: env) (e: exp):
+      (g ⊢ e ⊳* e)
   | R_Trans (g: env) (e e' e'': exp) :
-      RedClos g e e' ->
-      RedClos g e' e'' ->
-      RedClos g e e''
+      (g ⊢ e ⊳* e') ->
+      (g ⊢ e' ⊳* e'') ->
+      (g ⊢ e ⊳* e'')
   | R_CongLet (g: env) (e e': exp) (e1 e2 A: exp) (x: name) :
-      RedClos g e e' ->
-      RedClos (g & x ~ Def e A) (open x e1) (open x e2) -> (*FIXME: where does A come from *)
-      RedClos g (eLet e e1) (eLet e' e2) 
+      (g ⊢ e ⊳* e') ->
+      ((g & x ~ Def e A) ⊢ (open x e1) ⊳* (open x e2)) -> (*FIXME: where does A come from *)
+      (g ⊢ (eLet e e1) ⊳* (eLet e' e2))
   | R_CongLam1 (g: env) (A: exp) (A' e e': exp) (x: name)   :
-      RedClos g A A' ->
-      RedClos (g & x ~ Assum A) (open x e) (open x e') ->
-      RedClos g (eAbs A e) (eAbs A' e')
+      (g ⊢ A ⊳* A') ->
+      (g & x ~ Assum A ⊢ open x e ⊳* open x e') ->
+      (g ⊢ eAbs A e ⊳* eAbs A' e')
   | R_CongPi (g: env) (A: exp) (A' B B': exp) (x: name) :
-      RedClos g A A' ->
-      RedClos (g & x ~ Assum A) (open x B) (open x B') ->
-      RedClos g (ePi A B) (ePi A' B')
+      (g ⊢ A ⊳* A') ->
+      (g & x ~ Assum A ⊢ open x B ⊳* open x B') -> 
+      (g ⊢ ePi A B ⊳* ePi A' B')
   | R_CongSig (g: env) (A: exp) (A' B B': exp) (x: name) :
-      RedClos g A A' ->
-      RedClos (g & x ~ Assum A) (open x B) (open x B') ->
-      RedClos g (eSig A B) (eSig A' B')
+      (g ⊢ A ⊳* A') ->
+      (g & x ~ Assum A ⊢ open x B ⊳* open x B') -> 
+      (g ⊢ eSig A B ⊳* eSig A' B')
   | R_CongPair (g: env) (e1 e1' e2 e2' A A': exp) :
-      RedClos g e1 e1' ->
-      RedClos g e2 e2' ->
-      RedClos g A A'   ->
-      RedClos g (ePair e1 e2 A) (ePair e1' e2' A')
+      (g ⊢ e1 ⊳* e1') ->
+      (g ⊢ e2 ⊳* e2') -> 
+      (g ⊢ A ⊳* A') -> 
+      (g ⊢ ePair e1 e2 A ⊳* ePair e1' e2' A')
   | R_CongApp (g: env) (e1 e1' e2 e2': exp) :
-      RedClos g e1 e1' ->
-      RedClos g e2 e2' ->
-      RedClos g (eApp e1 e2) (eApp e1' e2')
+      (g ⊢ e1 ⊳* e1') -> 
+      (g ⊢ e2 ⊳* e2') -> 
+      (g ⊢ eApp e1 e2 ⊳* eApp e1' e2')
   | R_CongFst (g: env) (V V': exp) :
-      RedClos g V V' ->
-      RedClos g (eFst V) (eFst V')
+      (g ⊢ V ⊳* V') -> 
+      (g ⊢ eFst V ⊳* eFst V')
   | R_CongSnd (g: env) (V V': exp) :
-      RedClos g V V' ->
-      RedClos g (eSnd V) (eSnd V')
+      (g ⊢ V ⊳* V') -> 
+      (g ⊢ eSnd V ⊳* eSnd V')
   | R_CongIf (g: env) (e e' e1 e1' e2 e2': exp) :
-      RedClos g e e' ->
-      RedClos g e1 e1' ->
-      RedClos g e2 e2' ->
-      RedClos g (eIf e e1 e2) (eIf e' e1' e2')
-.
-Notation "g '|-' e1 '=r>' e2":= (RedClos g e1 e2) (at level 250, e1 at level 99): ECCA_scope.
+      (g ⊢ e ⊳* e') ->
+      (g ⊢ e1 ⊳* e1') -> 
+      (g ⊢ e2 ⊳* e2') -> 
+      (g ⊢ eIf e e1 e2 ⊳* eIf e' e1' e2')
+where "g '⊢' e1 '⊳*' e2":= (Reduces g e1 e2): ECCA_scope.
+
 (* TODO: rewrite with notation for readability *)
-Hint Constructors RedClos.
-Bind Scope ECCA_scope with RedClos.
+Hint Constructors Reduces.
+Bind Scope ECCA_scope with Reduces.
