ECCA/typing_lemmas.v
@@ -1,21 +1,47 @@
 Require Export typing.
 
-Open Scope ECCA_scope.
+(* Open Scope ECCA_scope.
 Theorem weakening {Γ e A}:
   (Γ |- e : A) ->
   forall r Δ,
     Γ =[r]=> Δ ->
     (Δ |- ([r] e) : A).
 Proof.
-Admitted.
+Admitted. *)
 
-Open Scope ECCA.
-Theorem backwards_reasoning_bool (g:env) (v: exp):
-((g |- v : eBool) ->
-((g |- v =r> eTru) \/ 
-(g |- v =r> eFls))).
+Lemma type_well_typed (g: env) (N: exp) (A: exp) :
+  Types g N A ->
+  WellFormed g ->
+  exists U , Types g A U.
 Proof.
-intros.
-inversion H; subst.
-+ inversion H0. (* With an id in the context, all we have is the type *)
-Abort.
+  induction 1.
+  - exists (eUni (uType 1)). apply aT_Ax_Type. auto.
+  - exists (eUni (uType (S (S i)))). apply aT_Ax_Type. auto.
+  - intros. induction H0.
+    + subst. destruct H; destruct h. 
+    + subst. destruct H. cbn in h. destruct (bindv (closev x0 x)).
+      * names.  
+  - exists (eUni (uType 1)). apply aT_Ax_Type. auto.
+  - exists (eUni (uType 0)). apply aT_Bool. auto.
+  - exists (eUni (uType 0)). apply aT_Bool. auto.
+  - apply IHTypes1.
+  - exists (eUni (uType 0)). eapply aT_Sig. shelve. shelve.
+  - exists (eUni (uType 0)). apply aT_Ax_Prop. shelve.
+  - exists (eUni (uType (S i))). apply aT_Ax_Type. shelve.
+  - exists (eUni (uProp)). eapply aT_Prod_Prop. shelve. shelve.
+  - shelve.
+  - shelve.
+  - exists U. auto.
+  - shelve.
+  - shelve.
+  - shelve. 
+Admitted. 
+
+Lemma has_type_wf_g (g: env) (N: exp) (A: exp) (x : name):
+  Types g N A ->
+  WellFormed g ->
+  WellFormed (g & x ~ (Def N A)).
+Proof.
+  intros.  apply type_well_typed in H as H1. destruct H1.
+  apply wf_Def with (U := x0); auto.
+Qed. 
